pancake/proofs/ntime_to_panProofScript.sml
@@ -1,0 +1,481 @@
+(*
+  Correctness proof for --
+*)
+
+open preamble
+     time_to_panProofTheory
+
+
+val _ = new_theory "ntime_to_panProof";
+
+val _ = set_grammar_ancestry
+        ["time_to_panProof"];
+
+
+Definition action_rel_def:
+  (action_rel (Input i) s (t:('a,time_input) panSem$state) =
+   input_rel t.locals i t.ffi.ffi_state) ∧
+  (action_rel (Output os) s t =
+   output_rel t.locals s.waitTime t.ffi.ffi_state)
+End
+
+
+Definition ffi_rel_def:
+  (ffi_rel (LDelay d) s (t:('a,time_input) panSem$state) =
+   ∃cycles.
+     delay_rep d t.ffi.ffi_state cycles ∧
+     wakeup_rel t.locals s.waitTime t.ffi.ffi_state cycles ∧
+     mem_read_ffi_results (:α) t.ffi.ffi_state cycles) ∧
+  (ffi_rel (LAction act) s t = action_rel act s t)
+End
+
+Definition local_action_def:
+  (local_action (Input i) t =
+     (FLOOKUP t.locals «isInput» = SOME (ValWord 0w))) ∧
+  (local_action (Output os) t =
+    (FLOOKUP t.locals «event»   = SOME (ValWord 0w) ∧
+     FLOOKUP t.locals «isInput» = SOME (ValWord 1w) ∧
+     FLOOKUP t.locals «waitSet» = SOME (ValWord 0w)))
+End
+
+Definition local_state_def:
+  (local_state (LDelay _) t =
+   (FLOOKUP t.locals «isInput» = SOME (ValWord 1w) ∧
+    FLOOKUP t.locals «event» = SOME (ValWord 0w))) ∧
+  (local_state (LAction act) t = local_action act t)
+End
+
+
+Definition event_state_def:
+  event_state t ⇔
+    FLOOKUP t.locals «isInput» = SOME (ValWord 1w) ∧
+    FLOOKUP t.locals «event»   =  SOME (ValWord 0w)
+End
+
+(* taken from the conclusion of individual step thorems *)
+Definition next_ffi_state_def:
+  (next_ffi_state (LDelay d) ffi (t:('a,time_input) panSem$state) ⇔
+   ∀cycles.
+     delay_rep d ffi cycles ⇒
+     t.ffi.ffi_state = nexts_ffi cycles ffi) ∧
+  (next_ffi_state (LAction _) ffi t ⇔ t.ffi.ffi_state = ffi)
+End
+
+(* pancake state only take ffi behaviour into account *)
+Definition ffi_rels_def:
+  (ffi_rels [] prog s (t:('a,time_input) panSem$state) ⇔ T) ∧
+  (ffi_rels (label::labels) prog s t ⇔
+   ∃ffi'.
+     ffi_rel label s t ffi' ∧
+     ∀s' t'.
+       step prog label s s' ∧
+       t'.ffi = ffi' ⇒
+       ffi_rels labels prog s' t')
+End
+
+Definition always_def:
+  always clksLength =
+  While (Const 1w)
+        (task_controller clksLength)
+End
+
+Theorem foo:
+  ∀prog s s' labels (t:('a,time_input) panSem$state).
+    stepTrace prog s s' labels ∧
+    state_rel (clksOf prog) s t ∧
+    code_installed t.code prog ∧
+    ffi_rels labels prog s t ∧
+    labProps$good_dimindex (:'a) ∧
+    (* everything is declared *)
+    (* add more updates later *) ⇒
+    ?ck t'.
+      evaluate (always (nClks prog), t with clock := t.clock + ck) =
+      evaluate (always (nClks prog), t') ∧
+      state_rel (clksOf prog) s' t' ∧
+      code_installed t'.code prog
+Proof
+QED
+
+
+
+
+
+(*
+Definition next_wakeup_def:
+  (next_wakeup (LDelay _) (t:('a,time_input) panSem$state) (t':('a,time_input) panSem$state) =
+   (FLOOKUP t'.locals «wakeUpAt» = FLOOKUP t.locals «wakeUpAt»)) ∧
+  (next_wakeup (LAction _) t t' =
+   (t'.ffi.ffi_state = t.ffi.ffi_state ∧
+    (∃wt.
+       FLOOKUP t'.locals «wakeUpAt» =
+       SOME (ValWord (n2w (FST (t.ffi.ffi_state 0) + wt))) ∧
+       FST (t.ffi.ffi_state 0) + wt < dimword (:α))))
+End
+*)
+
+
+(*
+Theorem step_thm:
+  !prog label s s' (t:('a,time_input) panSem$state) ck_extra.
+    step prog label s s' ∧
+    state_rel (clksOf prog) s t ∧
+    code_installed t.code prog ∧
+    labProps$good_dimindex (:'a) ⇒
+    case label of
+    | LDelay d =>
+        ∀cycles.
+          delay_rep (dimword (:α)) d t.ffi.ffi_state cycles ∧
+          wakeup_rel t.locals (dimword (:α)) s.waitTime t.ffi.ffi_state cycles ∧
+          mem_read_ffi_results (:α) t.ffi.ffi_state cycles ∧
+          FLOOKUP t.locals «isInput» = SOME (ValWord 1w) ⇒
+          ?ck t'.
+            evaluate (task_controller (nClks prog), t with clock := t.clock + ck) =
+            evaluate (task_controller (nClks prog), t' with clock := t'.clock + ck_extra) ∧
+            code_installed t'.code prog ∧
+            state_rel (clksOf prog) s' t' ∧
+            t'.ffi.ffi_state = nexts_ffi cycles t.ffi.ffi_state ∧
+            t'.ffi.oracle = t.ffi.oracle ∧
+            FLOOKUP t'.locals «wakeUpAt» = FLOOKUP t.locals «wakeUpAt» ∧
+            FLOOKUP t'.locals «isInput» = SOME (ValWord 1w) ∧
+            FLOOKUP t'.locals «sysTime»  =
+            SOME (ValWord (n2w (FST (t.ffi.ffi_state cycles))))
+    | LAction (Input i) =>
+        well_formed_terms prog s t ∧
+        input_rel t.locals (dimword (:α)) i t.ffi.ffi_state ∧
+        FLOOKUP t.locals «isInput» = SOME (ValWord 0w) ∧
+        task_ret_defined t.locals (nClks prog) ⇒
+        ?ck t'.
+          evaluate (task_controller (nClks prog), t with clock := t.clock + ck) =
+          (NONE, t') ∧
+          code_installed t'.code prog ∧
+          state_rel (clksOf prog) s' t' ∧
+          t'.ffi.ffi_state = t.ffi.ffi_state ∧
+          t'.ffi.oracle = t.ffi.oracle ∧
+          FLOOKUP t'.locals «sysTime» = FLOOKUP t.locals «sysTime» ∧
+          FLOOKUP t'.locals «event»   = SOME (ValWord 0w) ∧
+          FLOOKUP t'.locals «isInput» = SOME (ValWord 1w) ∧
+          task_ret_defined t'.locals (nClks prog) ∧
+          (∃wt.
+             FLOOKUP t'.locals «wakeUpAt» =
+             SOME (ValWord (n2w (FST (t.ffi.ffi_state 0) + wt))) ∧
+             FST (t.ffi.ffi_state 0) + wt < dimword (:α))
+    | LAction (Output os) =>
+        well_formed_terms prog s t ∧
+        output_rel t.locals (dimword (:α)) s.waitTime t.ffi.ffi_state ∧
+        FLOOKUP t.locals «event»   = SOME (ValWord 0w) ∧
+        FLOOKUP t.locals «isInput» = SOME (ValWord 1w) ∧
+        FLOOKUP t.locals «waitSet» = SOME (ValWord 0w) ∧
+        task_ret_defined t.locals (nClks prog) ∧
+        (∃tt. s.waitTime = SOME tt) ⇒
+        ?ck t'.
+          evaluate (task_controller (nClks prog), t with clock := t.clock + ck) =
+          (NONE, t') ∧
+          code_installed t'.code prog ∧
+          state_rel (clksOf prog) s' t' ∧
+          t'.ffi.ffi_state = t.ffi.ffi_state ∧
+          t'.ffi.oracle = t.ffi.oracle ∧
+          FLOOKUP t'.locals «sysTime» = FLOOKUP t.locals «sysTime» ∧
+          FLOOKUP t'.locals «event»   = SOME (ValWord 0w) ∧
+          FLOOKUP t'.locals «isInput» = SOME (ValWord 1w) ∧
+          task_ret_defined t'.locals (nClks prog) ∧
+          (∃wt.
+             FLOOKUP t'.locals «wakeUpAt» =
+             SOME (ValWord (n2w (FST (t.ffi.ffi_state 0) + wt))) ∧
+             FST (t.ffi.ffi_state 0) + wt < dimword (:α))
+Proof
+  rw [] >>
+  cases_on ‘label’ >>
+  fs []
+  >- (
+    rw [] >>
+    drule_all step_delay >>
+    disch_then (qspec_then ‘ck_extra’ mp_tac) >>
+    fs []) >>
+  cases_on ‘i’
+  >- (
+    fs [] >>
+    rw [] >>
+    drule_all step_input >>
+    disch_then (qspec_then ‘ck_extra’ mp_tac) >>
+    fs []) >>
+  fs [] >>
+  rw [] >>
+  drule step_output >>
+  disch_then (qspec_then ‘t’ mp_tac) >>
+  fs []
+QED
+*)
+
+
+
+
+(*
+Definition well_formness_def:
+  (well_formness (LDelay _) prog s (t:('a,time_input) panSem$state) = T) ∧
+  (well_formness (LAction _) prog s t =
+   (well_formed_terms prog s t ∧ task_ret_defined t.locals (nClks prog)))
+End
+*)
+
+
+
+Theorem step_delay_weaker:
+  !prog d s s' (t:('a,time_input) panSem$state).
+    step prog (LDelay d) s s' ∧
+    state_rel (clksOf prog) s t ∧
+    code_installed t.code prog ∧
+    ffi_rel (LDelay d) s t ∧
+    local_state (LDelay d) t ∧
+    code_installed t.code prog ∧
+    labProps$good_dimindex (:'a) ∧
+    (* extra assumptions *)
+    task_ret_defined t.locals (nClks prog) ∧
+    well_formed_terms prog s t ⇒
+    ?ck t'.
+      evaluate (task_controller (nClks prog), t with clock := t.clock + ck) =
+      evaluate (task_controller (nClks prog), t') ∧
+      state_rel (clksOf prog) s' t' ∧
+      code_installed t'.code prog ∧
+      next_wakeup (LDelay d) t t' ∧
+      event_state t' ∧
+      task_ret_defined t'.locals (nClks prog) ∧
+      well_formed_terms prog s' t'
+Proof
+  rw [] >>
+  fs [ffi_rel_def] >>
+  drule step_delay >>
+  disch_then (qspecl_then [‘cycles’, ‘t’, ‘0’] mp_tac) >>
+  impl_tac
+  >- gs [local_state_def] >>
+  strip_tac >>
+  qexists_tac ‘ck’ >>
+  qexists_tac ‘t'’ >>
+  gs [] >>
+  ‘t' with clock := t'.clock = t'’ by
+    fs [state_component_equality] >>
+  gs [next_wakeup_def, event_state_def, local_state_def] >>
+  gs [task_ret_defined_def] >>
+  fs [step_cases]
+  >- (
+    gs [well_formed_terms_def, mkState_def] >>
+    gen_tac >>
+    strip_tac >>
+    first_x_assum drule >>
+    strip_tac >>
+    gs [resetOutput_def] >>
+    conj_tac
+    >- (
+      gs [conds_eval_lt_dimword_def] >>
+      gs [EVERY_MEM] >>
+      rw [] >>
+      first_x_assum drule_all >>
+      gs []  >>
+      TOP_CASE_TAC >> gs [] >>
+      strip_tac >>
+      cheat) >>
+    (* this is complicated *)
+    conj_tac
+    >- cheat >>
+    cheat) >>
+  cheat
+QED
+
+Theorem step_input_weaker:
+  !prog i s s' (t:('a,time_input) panSem$state).
+    step prog (LAction (Input i)) s s' ∧
+    state_rel (clksOf prog) s t ∧
+    code_installed t.code prog ∧
+    ffi_rel (LAction (Input i)) s t ∧
+    local_state (LAction (Input i)) t ∧
+    code_installed t.code prog ∧
+    labProps$good_dimindex (:'a) ∧
+    (* extra assumptions *)
+    task_ret_defined t.locals (nClks prog) ∧
+    well_formed_terms prog s t ⇒
+    ?ck t'.
+      evaluate (task_controller (nClks prog), t with clock := t.clock + ck) =
+      (NONE, t') ∧
+      state_rel (clksOf prog) s' t' ∧
+      code_installed t'.code prog ∧
+      next_wakeup (LAction (Input i)) t t' ∧
+      event_state t' ∧
+      task_ret_defined t'.locals (nClks prog) ∧
+      well_formed_terms prog s' t'
+Proof
+  rw [] >>
+  fs [ffi_rel_def] >>
+  drule step_input >>
+  disch_then (qspec_then ‘t’ mp_tac) >>
+  impl_tac
+  >- gs [action_rel_def, local_state_def, local_action_def] >>
+  strip_tac >>
+  qexists_tac ‘ck’ >>
+  qexists_tac ‘t'’ >>
+  gs [] >>
+  conj_tac
+  >- (
+    gs [next_wakeup_def] >>
+    qexists_tac ‘wt’ >> gs []) >>
+  conj_tac
+  >- gs [event_state_def] >>
+  gs [well_formed_terms_def]  >>
+  gen_tac >>
+  strip_tac >>
+  (* need more assumptions *)
+  cheat
+QED
+
+
+Theorem step_output_weaker:
+  !prog os s s' (t:('a,time_input) panSem$state).
+    step prog (LAction (Output os)) s s' ∧
+    state_rel (clksOf prog) s t ∧
+    code_installed t.code prog ∧
+    ffi_rel (LAction (Output os)) s t ∧
+    local_state (LAction (Output os)) t ∧
+    code_installed t.code prog ∧
+    labProps$good_dimindex (:'a) ∧
+    (* should be rephrased *)
+    (∃tt. s.waitTime = SOME tt) ∧
+    (* extra assumptions *)
+    task_ret_defined t.locals (nClks prog) ∧
+    well_formed_terms prog s t ⇒
+    ?ck t'.
+      evaluate (task_controller (nClks prog), t with clock := t.clock + ck) =
+      (NONE, t') ∧
+      state_rel (clksOf prog) s' t' ∧
+      code_installed t'.code prog ∧
+      next_wakeup (LAction (Output os)) t t' ∧
+      event_state t' ∧
+      task_ret_defined t'.locals (nClks prog) ∧
+      well_formed_terms prog s' t'
+Proof
+  rw [] >>
+  fs [ffi_rel_def] >>
+  drule step_output >>
+  disch_then (qspec_then ‘t’ mp_tac) >>
+  impl_tac
+  >- gs [action_rel_def, local_state_def, local_action_def] >>
+  strip_tac >>
+  qexists_tac ‘ck’ >>
+  qexists_tac ‘t'’ >>
+  gs [] >>
+  conj_tac
+  >- (
+    gs [next_wakeup_def] >>
+    qexists_tac ‘wt’ >> gs []) >>
+  conj_tac
+  >- gs [event_state_def] >>
+  gs [well_formed_terms_def]  >>
+  gen_tac >>
+  strip_tac >>
+  (* need more assumptions *)
+  cheat
+QED
+
+
+(*
+Definition next_wakeup_def:
+  (next_wakeup (LDelay _) (t:('a,time_input) panSem$state) (t':('a,time_input) panSem$state) =
+   (FLOOKUP t'.locals «waitSet» = SOME (ValWord 0w) ∧
+    FLOOKUP t'.locals «wakeUpAt» = FLOOKUP t.locals «wakeUpAt»)) ∧
+  (next_wakeup (LAction _) t t' =
+   (t'.ffi.ffi_state = t.ffi.ffi_state ∧
+    FLOOKUP t'.locals «waitSet» = SOME (ValWord 0w) ∧
+    (∃wt.
+       FLOOKUP t'.locals «wakeUpAt» =
+       SOME (ValWord (n2w (FST (t.ffi.ffi_state 0) + wt))) ∧
+       FST (t.ffi.ffi_state 0) + wt < dimword (:α))))
+End
+
+
+Definition eventual_wakeup_def:
+  eventual_wakeup prog <=>
+  let tms = FLAT (MAP SND prog) in
+    EVERY (λtm.
+            ∃h t. termWaitTimes tm = h::t)
+          tms
+End
+*)
+
+
+
+(* start from here *)
+(*
+ While (Const 1w)
+             (task_controller clksLength)
+*)
+(* should we talk about number of states, more like a trace
+   sts: list of reachable timeSem state
+   ts: list of states,
+
+   what exactly do we need∃ *)
+Theorem foo:
+  ∀prog s s' labels (t:('a,time_input) panSem$state).
+    stepTrace prog s s' labels ∧
+    state_rel (clksOf prog) s t ∧
+    code_installed t.code prog ∧
+    ffi_rels labels prog s t ∧
+    labProps$good_dimindex (:'a) ∧
+    (* everything is declared *)
+    (* add more updates later *) ⇒
+    ?ck t'.
+      evaluate (always (nClks prog), t with clock := t.clock + ck) =
+      evaluate (always (nClks prog), t') ∧
+      state_rel (clksOf prog) s' t' ∧
+      code_installed t'.code prog
+Proof
+QED
+
+
+
+
+
+
+
+
+
+
+
+
+
+
+
+
+
+
+
+
+
+
+
+
+
+
+
+
+
+
+
+
+
+
+
+
+
+
+
+
+
+
+
+
+
+
+
+
+
+
+
+
+val _ = export_theory();
